Drastically simplify the proofs of getAndSet

formal-proofs/theories/lib/util/getAndSet.v
@@ -1,116 +1,34 @@
 From iris.base_logic.lib Require Export invariants.
 From iris.proofmode Require Import tactics.
 From iris.heap_lang Require Import proofmode notation lang.
-From iris.program_logic Require Export weakestpre atomic.
+From iris.program_logic Require Export atomic.
+
+Definition getAndSet : val :=
+  rec: "getAndSet" "l" "v" :=
+    let: "o" := ! "l" in
+    if: CAS "l" "o" "v"
+    then "o"
+    else "getAndSet" "l" "v".
 
 Section getAndSetProof.
 
 Context `{heapG} (N: namespace).
 
-Definition getAndSetInner : val :=
-  rec: "getAndSet" "p" "g" "l" "v" "o" :=
-    let: "r" := Resolve (CmpXchg "l" "o" "v") "p" "g" in
-    if: Snd "r"
-    then "o"
-    else "getAndSet" "p" "g" "l" "v" (Fst "r").
-
-Definition getAndSet : val :=
-  λ: "l" "v",
-  let: "p" := NewProph in
-  let: "g" := ref #() in
-    getAndSetInner "p" "g" "l" "v" #0.
-
-Theorem getAndSet_spec : forall (ℓ: loc) v, val_is_unboxed v ->
-  inv N (∃ v, ℓ ↦{1/2} v ∧ ⌜val_is_unboxed v⌝) -∗
-  <<< ∀ k, ℓ ↦{1/2} k >>>
+Theorem getAndSet_spec (ℓ: loc) (v: val):
+  <<< ∀ k, ℓ ↦ k ∧ ⌜val_is_unboxed k⌝>>>
     getAndSet #ℓ v @ ⊤ ∖ ↑N
-  <<< ℓ ↦{1/2} v, RET k >>>.
+  <<< ℓ ↦ v, RET k >>>.
 Proof.
-  iIntros (ℓ v v_unboxed) "#HInv".
-  iIntros (Φ) "AU".
-  wp_lam.
-  wp_let.
-  wp_bind NewProph.
-  wp_apply wp_new_proph; auto.
-  iIntros (pvs p) "HProph".
-  remember #0 as o.
-  assert (val_is_unboxed o) as o_unboxed by (subst; done).
-  clear Heqo.
-  wp_let.
-  wp_bind (ref _)%E.
-  wp_alloc lg_ghost as "Hghost".
-  wp_let.
-  iLöb as "IH" forall (o pvs o_unboxed).
-  wp_rec.
-  wp_pures.
-  wp_bind (Resolve _ _ _)%E.
-  iInv N as "Hℓ" "HClose".
-  iDestruct "Hℓ" as (trueVal) ">[Hℓ %]".
-  destruct pvs.
-  - iMod "AU" as (k) "[HAU [_ HCloseAU]]".
-    iDestruct (mapsto_combine with "HAU Hℓ") as "[Hℓ <-]".
-    replace (1 / 2 + 1 / 2)%Qp with 1%Qp by (rewrite Qp_half_half; done).
-    destruct (decide (o = k)); subst.
-    * wp_apply (wp_resolve_cmpxchg_suc with "[HProph Hℓ]"); auto.
-      + left; done.
-      + iFrame.
-      + iIntros "Hpvs'".
-        iDestruct "Hpvs'" as (pvs') "[% _]".
-        discriminate.
-    * wp_apply (wp_resolve_cmpxchg_fail with "[HProph Hℓ]"); eauto with iFrame.
-      + right; done.
-      + iIntros "Hpvs'". iDestruct "Hpvs'" as (pvs') "[% _]".
-        discriminate.
-  - destruct (decide (p0 = ((o, #true)%V, #lg_ghost))).
-    * subst.
-      iMod "AU" as (k) "[HAU [_ HCloseAU]]".
-      iDestruct (mapsto_combine with "HAU Hℓ") as "[Hℓ <-]".
-      replace (1 / 2 + 1 / 2)%Qp with 1%Qp by (rewrite Qp_half_half; done).
-      destruct (decide (o = k)); subst.
-      2: {
-        wp_apply (wp_resolve_cmpxchg_fail with "[HProph Hℓ]"); eauto with iFrame.
-        + right; done.
-        + iIntros "Hpvs'". iDestruct "Hpvs'" as (pvs') "[% _]".
-          discriminate.
-      }
-      wp_apply (wp_resolve_cmpxchg_suc with "[HProph Hℓ]"); eauto with iFrame.
-      { right; done. }
-      iIntros "Hpvs'". iDestruct "Hpvs'" as (pvs') "[% [HProph Hℓ]]".
-      replace (ℓ ↦ v)%I with (ℓ ↦{1/2 + 1/2} v)%I by (rewrite Qp_half_half; done).
-      inversion H1; subst. clear H1.
-      iDestruct "Hℓ" as "[Hℓ1 Hℓ2]".
-      iMod ("HCloseAU" with "Hℓ1") as "HΦ".
-      iModIntro.
-      iMod ("HClose" with "[Hℓ2]") as "_"; first by (eauto with iFrame).
-      iModIntro.
-      wp_pures.
-      auto.
-    * destruct (decide (o = trueVal)).
-      {
-        iMod "AU" as (k) "[HAU [_ HCloseAU]]".
-        iDestruct (mapsto_combine with "HAU Hℓ") as "[Hℓ <-]".
-        replace (1 / 2 + 1 / 2)%Qp with 1%Qp by (rewrite Qp_half_half; done).
-        wp_apply (wp_resolve_cmpxchg_suc with "[HProph Hℓ]"); eauto with iFrame.
-        { right; done. }
-        { subst; iFrame. }
-        iIntros "Hpvs'". iDestruct "Hpvs'" as (pvs') "[% [HProph Hℓ]]".
-        inversion H1.
-        subst.
-        contradiction.
-      }
-      wp_apply (wp_resolve_cmpxchg_fail with "[HProph Hℓ]"); eauto with iFrame.
-      { right; done. }
-      iIntros "Hpvs'". iDestruct "Hpvs'" as (pvs') "[% [HProph Hℓ]]".
-      iMod ("HClose" with "[Hℓ]") as "_"; first by auto.
-      iModIntro.
-      wp_let.
-      wp_proj.
-      wp_if.
-      wp_proj.
-      iSpecialize ("IH" $! trueVal pvs' H0).
-      clear.
-      iSpecialize ("IH" with "AU HProph Hghost").
-      wp_apply "IH".
+  iIntros (Φ) "AU". iLöb as "IH". wp_lam. wp_pures.
+  wp_bind (!_)%E. iMod "AU" as (k) "[[Hℓ %] [HClose _]]".
+  wp_load. iMod ("HClose" with "[Hℓ]") as "AU"; first by iSplit. iModIntro.
+  wp_let. wp_bind (CmpXchg _ _ _)%E. iMod "AU" as (k') "[[Hℓ %] HClose]".
+  destruct (decide (k = k')) as [[= ->]|Hx];
+    [wp_cmpxchg_suc|wp_cmpxchg_fail];
+    [iDestruct "HClose" as "[_ HClose]" | iDestruct "HClose" as "[HClose _]"].
+  all: iMod ("HClose" with "[Hℓ]") as "HΦ"; first by auto.
+  all: iModIntro; wp_pures; auto.
+  by wp_apply "IH".
 Qed.
 
 End getAndSetProof.
